examples/low-level/crypto/Crypto.Symmetric.MAC.fst
@@ -1,0 +1,138 @@
+module Crypto.Symmetric.MAC
+
+open Crypto.Symmetric.Bytes
+open Flag
+
+module GF = Crypto.Symmetric.GF128
+module PLS = Crypto.Symmetric.Poly1305.Spec
+module PL = Crypto.Symmetric.Poly1305
+
+module HH = FStar.HyperHeap
+module HS = FStar.HyperStack
+
+type elem128 = lbytes 16
+
+let alg i = Flag.mac_of_id i 
+
+(* this file multiplexes between different real implementations of
+   polynomial MACs. It is indifferent to the static vs one-time 
+   allocation of the r part of the key *)
+
+let elem i = 
+  match alg i with
+  | POLY1305 -> PLS.elem
+  | GHASH    -> elem128
+
+let elemB i = 
+  b: Buffer.buffer 
+    (if alg i = POLY1305 then UInt64.t else UInt8.t) 
+    {Buffer.length b = (if alg i = POLY1305 then 5 else 16)}
+//  match alg i with
+//  | POLY1305 -> PL.elemB
+//  | GHASH    -> lbuffer 16
+
+let live h #i (b:elemB i) = 
+  match alg i with
+  | POLY1305 -> Buffer.live #UInt64.t h b /\ 
+               //16-10-17 annoying; implying live.
+               Crypto.Symmetric.Poly1305.Bigint.norm h b
+  | GHASH    -> Buffer.live #UInt8.t h b
+
+let rcreate (rgn:HH.rid{HS.is_eternal_region rgn}) i: ST (elemB i)
+  (requires (fun h0 -> True))
+  (ensures (fun h0 r h1 ->
+    HS.modifies (Set.singleton rgn) h0 h1 /\
+    HS.modifies_ref rgn TSet.empty h0 h1 
+  )) =   
+  match alg i with 
+  | POLY1305 -> FStar.Buffer.rcreate rgn 0UL 5ul
+  | GHASH    -> FStar.Buffer.rcreate rgn 0uy 16ul
+
+let create i : StackInline (elemB i) 
+  (requires (fun h0 -> True))
+  (ensures (fun h0 r h1 ->
+    Buffer.modifies_0 h0 h1
+  )) = 
+  match alg i with 
+  | POLY1305 -> FStar.Buffer.create 0UL 5ul
+  | GHASH    -> FStar.Buffer.create 0uy 16ul
+
+(* avoiding:
+let frameOf #i (b:elemB i) = 
+  match alg i with
+  | POLY1305 -> Buffer.frameOf #UInt64.t b
+  | GHASH    -> Buffer.frameOf #UInt8.t b
+*)
+
+let sel_elem h #i (b:elemB i{live h b}) : elem i =
+  match alg i with 
+  | POLY1305 -> PL.sel_elem h b
+  | GHASH    -> Buffer.as_seq #UInt8.t h b 
+
+
+let encode_r i (b:elemB i) (raw:lbuffer 16) = 
+  match alg i with 
+  | POLY1305 -> PL.clamp raw; 
+               PL.toField b raw
+  | GHASH    -> Buffer.blit raw 0ul b 0ul 16ul
+
+let encode h i (w:lbytes 16): elem i = 
+  match alg i with 
+  | POLY1305 -> PLS.encode w
+  | GHASH    -> w 
+
+(*
+let mac i (log:Seq.seq (elem i)) (r:elem i) (s:lbytes 16) : Tot (lbytes 16) = 
+  match alg i with
+  | POLY1305 -> PLS.mac_1305 log r s 
+  | GHASH    -> admit()
+*)
+
+private let encodeB i w : elemB i = 
+  match alg i with 
+  | POLY1305 -> let b = Buffer.create 0UL 5ul in 
+               PL.toField_plus_2_128 b w;
+               b
+  | GHASH    -> w 
+
+assume val gf128_poly: cs:Seq.seq elem128 -> r:elem128 -> Tot elem128
+
+(* we also need an abstract polynomial-evaluation spec *)
+//16-10-17  removing abstraction for now
+let poly #i (cs:Seq.seq (elem i)) (r:elem i) : elem i = 
+  match alg i with 
+  | POLY1305 -> PLS.poly cs r 
+  | GHASH    -> gf128_poly cs r
+
+let start i = create i 
+  
+let update #i (r: elemB i) (a:elemB i) (w:lbuffer 16) = 
+  push_frame();
+  let e = encodeB i w in 
+  match alg i with 
+  | POLY1305 -> PL.add_and_multiply a e r (* to be adapted from poly1305.mac *)
+  | GHASH    -> GF.add_and_multiply a w r;
+  pop_frame()
+  (* TODO: re-use the elem buffer 
+     rather that create a fresh one, maybe in the accumulator *)
+
+let finish i (s:lbuffer 16) (a:elemB i) (tag:lbuffer 16) = 
+  match alg i with 
+  | POLY1305 -> PL.poly1305_finish tag a s
+  | GHASH    -> GF.gf128_add a s; 
+               Buffer.blit a 0ul tag 0ul 16ul
+
+      
+
+  
+
+
+  
+
+
+
+
+
+
+
+
